Moved files around: LDef.v and LProps.v to "O..." versions and RecordExt.v to LDef.v and LProps.v.  Changed the headers of other files accordingly.

LDef.v
@@ -1,154 +1,129 @@
-(** * LDef: Definition of an STLC-based language.  *)
+(** * LDef: STLC with records (as lists). *)
 
-(** This is SF's Stlc with Gamma change to be a list of declarations.
-*)
+(** This file started out as SF's Records.v but has been modified to 
+    have records as lists of declarations. 
+    This is in contrast to SF's approach. *)
 
 Load Init.
 Require Export SfLib.
 Require Import LibTactics.
 
+Require Export Common.
+Import P3Common.
+
 Module LDEF.
 
 (* ###################################################################### *)
-(** ** Syntax *)
 
+(**  ** SYNTAX:
+<<
+       t ::=                          Terms:
+           | true, false                 boolean values
+           | x                           variable
+           | t1 t2                       application
+           | \x:T1.t2                    abstraction
+           | {F1; ...; Fn}               record 
+           | t.i                         projection
+           | if tb then te else tf       conditional
+       T ::=                          Types:
+           | X                           type variable (not used)
+           | Bool                        boolean type
+           | T1 -> T2                    function type
+           | {L1; ...; Ln}               record type
+       F ::=                          Definitions:
+           | val x = t                   bind value to id
+       L ::=                          Declarations:
+           | val x : T                   id has type
+>> 
+*)
 
-(* ################################### *)
-(** *** Types *)
+(**  *** Types [ty] *)
 
-Inductive ty : Type := 
-  | TBool  : ty 
-  | TArrow : ty -> ty -> ty.
+Inductive ty : Type :=
+  | TBase     : id -> ty
+  | TBool     : ty
+  | TArrow    : ty -> ty -> ty
+  | TRcd      : (list decl) -> ty
+with decl : Type :=
+  | Lv        : id -> ty -> decl.
 
-(* ################################### *)
-(** *** Terms *)
+(** *** Terms [tm] *)
 
 Inductive tm : Type :=
-  | tvar : id -> tm
-  | tapp : tm -> tm -> tm
-  | tabs : id -> ty -> tm -> tm
   | ttrue : tm
   | tfalse : tm
-  | tif : tm -> tm -> tm -> tm.
+  | tvar  : id -> tm
+  | tapp  : tm -> tm -> tm
+  | tabs  : id -> ty -> tm -> tm
+  | trcd  : list def -> tm
+  | tproj : tm -> id -> tm
+  | tif : tm -> tm -> tm -> tm
+with def : Type :=
+  | Fv    : id -> tm -> def.
+
+(** In SF there is an observation about how an embedded list doesn't 
+    give a useful induction principle, so they have
+    the following for types:
+<<
+      | TRNil : ty
+      | TRCons : id -> ty -> ty -> ty
+>>
+    Since this allows TRCons to be applied to non-record components,
+    they have a way to tell whether types are well-formed.  The same
+    thing applies to terms.
+
+    Instead, we use a list of declarations and fix the induction 
+    principle.  Similarly, record terms will be lists of definitions.
+*)
+
+(** *** "Case" tactic notations *)
+
+Tactic Notation "T_cases" tactic(first) ident(c) :=
+  first;
+  [ Case_aux c "TBase" | Case_aux c "TBool" 
+  | Case_aux c "TArrow" | Case_aux c "TRcd" ].
 
 Tactic Notation "t_cases" tactic(first) ident(c) :=
   first;
-  [ Case_aux c "tvar" | Case_aux c "tapp" 
-  | Case_aux c "tabs" | Case_aux c "ttrue" 
-  | Case_aux c "tfalse" | Case_aux c "tif" ].
+  [ Case_aux c "ttrue" | Case_aux c "tfalse" 
+  | Case_aux c "tvar" | Case_aux c "tapp" | Case_aux c "tabs"
+  | Case_aux c "trcd" | Case_aux c "tproj"| Case_aux c "tif" ].
 
 
+(** *** Functions and lemmas for dealing with definition and declaration lists *)
 
-(* ###################################################################### *)
-(** ** Operational Semantics *)
+Definition add_vdef x t Fs := (Fv x t) :: Fs.
+Definition add_vdecl x T Ls := (Lv x T) :: Ls.
 
-(* ################################### *)
-(** *** Values *)
-
-Inductive value : tm -> Prop :=
-  | v_abs : forall x T t,
-      value (tabs x T t)
-  | v_true : 
-      value ttrue
-  | v_false : 
-      value tfalse.
-
-Hint Constructors value.
-
-(* ###################################################################### *)
-(** *** Substitution *)
-
-Reserved Notation "'[' x ':=' s ']' t" (at level 20).
-
-Fixpoint subst (x:id) (s:tm) (t:tm) : tm :=
-  match t with
-  | tvar x' => 
-      if eq_id_dec x x' then s else t
-  | tabs x' T t1 => 
-      tabs x' T (if eq_id_dec x x' then t1 else ([x:=s] t1)) 
-  | tapp t1 t2 => 
-      tapp ([x:=s] t1) ([x:=s] t2)
-  | ttrue => 
-      ttrue
-  | tfalse => 
-      tfalse
-  | tif t1 t2 t3 => 
-      tif ([x:=s] t1) ([x:=s] t2) ([x:=s] t3)
-  end
-
-where "'[' x ':=' s ']' t" := (subst x s t).
-
-(** _Technical note_: Substitution becomes trickier to define if we
-    consider the case where [s], the term being substituted for a
-    variable in some other term, may itself contain free variables.
-    Since we are only interested here in defining the [step] relation
-    on closed terms (i.e., terms like [\x:Bool. x], that do not mention
-    variables are not bound by some enclosing lambda), we can skip
-    this extra complexity here, but it must be dealt with when
-    formalizing richer languages. *)
-
-
-(* ################################### *)
-(** *** Reduction *)
-
-Reserved Notation "t1 '==>' t2" (at level 40).
-
-Inductive step : tm -> tm -> Prop :=
-  | ST_AppAbs : forall x T t12 v2,
-         value v2 ->
-         (tapp (tabs x T t12) v2) ==> [x:=v2]t12
-  | ST_App1 : forall t1 t1' t2,
-         t1 ==> t1' ->
-         tapp t1 t2 ==> tapp t1' t2
-  | ST_App2 : forall v1 t2 t2',
-         value v1 ->
-         t2 ==> t2' -> 
-         tapp v1 t2 ==> tapp v1  t2'
-  | ST_IfTrue : forall t1 t2,
-      (tif ttrue t1 t2) ==> t1
-  | ST_IfFalse : forall t1 t2,
-      (tif tfalse t1 t2) ==> t2
-  | ST_If : forall t1 t1' t2 t3,
-      t1 ==> t1' ->
-      (tif t1 t2 t3) ==> (tif t1' t2 t3)
-
-where "t1 '==>' t2" := (step t1 t2).
-
-Tactic Notation "step_cases" tactic(first) ident(c) :=
-  first;
-  [ Case_aux c "ST_AppAbs" | Case_aux c "ST_App1" 
-  | Case_aux c "ST_App2" | Case_aux c "ST_IfTrue" 
-  | Case_aux c "ST_IfFalse" | Case_aux c "ST_If" ].
-
-Hint Constructors step.
-
-Notation multistep := (multi step).
-Notation "t1 '==>*' t2" := (multistep t1 t2) (at level 40).
-
-Tactic Notation "print_goal" := match goal with |- ?x => idtac x end.
-Tactic Notation "normalize" := 
-   repeat (print_goal; eapply multi_step ; 
-             [ (eauto 10; fail) | (instantiate; simpl)]);
-   apply multi_refl.
-
-(* ###################################################################### *)
-(** ** Typing *)
-
-(* ################################### *)
-(** *** Contexts *)
-
-Inductive decl :=
-  | Lv : id -> ty -> decl.
-
-Definition context := list decl.
-Definition empty := nil (A:=decl).
-Definition add_vdecl(x : id) (T : ty)  (Gamma : context) 
-  := (Lv x T) :: Gamma.
-Fixpoint lookup_vdecl (x : id) (Gamma : context) := 
-  match Gamma with 
+Fixpoint lookup_vdef x Fs := 
+  match Fs with 
     | nil => None 
-    | (Lv y T) :: Ls' => if eq_id_dec y x then Some T else lookup_vdecl x Ls'
+    | (Fv y t) :: Fs' => 
+        if eq_id_dec y x then Some t else lookup_vdef x Fs'
+    (* | _ :: Fs' => lookup_vdef x Fs' *)
   end.
+
+Fixpoint lookup_vdecl x Ls := 
+  match Ls with 
+    | nil => None 
+    | (Lv y T) :: Ls' => 
+        if eq_id_dec y x then Some T else lookup_vdecl x Ls'
+  end.
+
+Lemma lookup_add_vdef_eq : 
+  forall (x : id) (t : tm) (Fs : list def),
+    lookup_vdef x (add_vdef x t Fs) = Some t.
+Proof.
+  intros. simpl. apply eq_id.
+Qed.
+
+Lemma lookup_add_vdef_neq :
+  forall (x y : id) (t : tm) (Fs : list def),
+    y <> x ->
+    lookup_vdef x (add_vdef y t Fs) = lookup_vdef x Fs.
+Proof.
+  intros. simpl. apply neq_id. apply H.
+Qed.
 
 Lemma lookup_add_vdecl_eq : 
   forall (x : id) (T : ty) (Ls : list decl),
@@ -165,44 +140,582 @@ Proof.
   intros. simpl. apply neq_id. apply H.
 Qed.
 
-(*
-Lemma add_vdecl_eq : forall (ctxt: context) x T,
-  lookup_vdecl x (add_vdecl ctxt x T) = Some T.
-Proof.
-  intros. unfold add_vdecl, lookup_vdecl. rewrite eq_id; auto. 
-Qed.
+(* TBD: Try some of these attempts at making the above more generic:
 
-Lemma add_vdecl_neq : forall (ctxt: context) x1 x2 T,
-  x2 <> x1 ->
-  lookup_vdecl x1 (add_vdecl ctxt x2 T) = lookup_vdecl x1 ctxt.
-Proof.
-  intros. unfold add_vdecl, lookup_vdecl. rewrite neq_id; auto. 
-Qed.
+Definition lookup_generic {T U : Type} 
+    (extrf : T -> option U) (xs : list T) : option U := 
+  match xs with 
+    | nil => None
+    | x :: xs' => 
+      match extrf x with
+        | None => lookup_generic extrf xs'
+        | Some v => Some v
+      end
+  end.
+
+Definition vdef_xf (x : id) (vd : def) : option tm :=
+  match vd with 
+    | (Vd y t) => if id_eq_dec x y then Some t else None
+    | _ => None
+  end.
+Definition lookup_vdef x Fs := lookup_generic (vdef_xf x) Fs.
+
+Definition unapply_vdef (vd : vdef) : option (id * tm) :=
+  match vd with (Fv y t) => Some (y, t) | _ => None end.
+  
+Definition lookup_gen {T U : Type} (unapplyf : T -> option (id * U)) 
+    (x : id) (ts : list T) : option U :=
+  match ts with
+    | nil => None
+    | t : ts' => 
+      match unapplyf t with
+        | Some (y v) => 
+            if id_eq_dec x y then Some v else lookup_gen unapplyf x ts'
+        | None => lookup_gen unapplyf x ts'
+      end
+  end.
+Definition lookup_vdef := lookup_gen unapply_vdef.
 *)
 
-Lemma lookup_add_vdecl_shadow : forall (ctxt: context) t1 t2 x1 x2,
-  lookup_vdecl x1 (add_vdecl x2 t2 (add_vdecl x2 t1 ctxt))  
-    = lookup_vdecl x1 (add_vdecl x2 t2 ctxt).
-Proof with auto.
-  intros. unfold add_vdecl, lookup_vdecl. destruct (eq_id_dec x2 x1)...
+
+(* ###################################################################### *)
+(** ** Custom recursion principles. *)
+
+(** *** Recursion on types, [ty_nested_rect]
+
+    The coq-generated recursion function has the following type:
+<< 
+  ty_rect : 
+    forall P : ty -> Type,
+      (forall i : id, P (TBase i)) ->
+      P TBool ->
+      (forall t : ty, P t -> forall t0 : ty, P t0 -> P (TArrow t t0)) ->
+      (forall r : list decl, P (TRcd r)) -> (* records *)
+    forall t : ty, P t
+>>
+
+    The following custom recursion function replaces the last case 
+    (a proof of [P (TRcd r)] given only that [r : list decl])
+    with four:
+      - an additional proposition function [Q] over [list decl] (at the top),
+      - a proof that for record body type, [Trb], [Q Trb] implies [P (TRcd Trb)],
+      - a proof of [Q nil] and
+      - a proof that [P T] and [Q Trb] implies [Q (cons x T Trb))]
+
+    The definition may be a little hard to follow, as it is using the 
+    coq-generated [ty_rect] and [list_rect].  
+    The primed version should be the same thing using match expressions.
+*)
+
+Definition ty_nested_rect
+  (P: ty -> Type) 
+  (Q: list decl -> Type)
+    (fTBase : forall x : id, P (TBase x))
+    (fTBool : P (TBool))
+    (fTArrow : forall T1 : ty, P T1 -> forall T2 : ty, P T2 -> P (TArrow T1 T2))
+    (fTRcd' : forall Trb : list decl, Q Trb -> P (TRcd Trb))
+      (fTRcd_nil' : Q nil)
+      (fTRcd_cons' : forall (x : id) (T : ty) (Trb : list decl), 
+                       P T -> Q Trb -> Q ((Lv x T) :: Trb))
+  : forall T : ty, P T
+  := fix F (T : ty) : P T :=
+    let fTRcd_cons b Trb := 
+      match b with (Lv x T) => fTRcd_cons' x T Trb (F T) end
+    in let fTRcd Trb := fTRcd' Trb (list_rect Q fTRcd_nil' fTRcd_cons Trb)
+    in ty_rect P fTBase fTBool fTArrow fTRcd T.
+
+Definition ty_nested_rect'
+  (P: ty -> Type) 
+  (Q: list decl -> Type)
+    (fTBase : forall x : id, P (TBase x))
+    (fTBool : P (TBool))
+    (fTArrow : forall T1 : ty, P T1 -> forall T2 : ty, P T2 -> P (TArrow T1 T2))
+    (fTRcd' : forall Trb : list decl, Q Trb -> P (TRcd Trb))
+      (fTRcd_nil' : Q nil)
+      (fTRcd_cons' : forall (x : id) (T : ty) (Trb : list decl), 
+                       P T -> Q Trb -> Q ((Lv x T) :: Trb))
+  : forall T : ty, P T
+  := fix F (T : ty) : P T :=
+     let fix G (Trb : list decl) : Q Trb :=
+         match Trb with
+           | nil => fTRcd_nil'
+           | (Lv x T) :: Trb' => fTRcd_cons' x T Trb' (F T) (G Trb')
+         end
+     in match T with
+       | TBase x => fTBase x
+       | TBool => fTBool
+       | TArrow T1 T2 => fTArrow T1 (F T1) T2 (F T2)
+       | TRcd Trb => fTRcd' Trb (G Trb)
+     end.
+
+(* An attempt to do it as a Lemma, but the lack of a good IH kills it.
+
+Lemma ty_nested_rect'' :
+  forall 
+    (P: ty -> Type) 
+    (Q: list decl -> Type),
+    (forall x : id, P (TBase x)) ->
+    (forall T1 : ty, P T1 -> forall T2 : ty, P T2 -> P (TArrow T1 T2)) ->
+    (forall Trb : list decl, Q Trb -> P (TRcd Trb)) ->
+      (Q nil) ->
+      (forall (x : id) (T : ty) (Trb : list decl), 
+           P T -> Q Trb -> Q ((x, T) :: Trb)) ->
+  forall T : ty, P T.
+Proof.
+  intros P Q Hbase Harrow Hrcd Hnil Hcons T.
+  T_cases (induction T) Case; auto.
+    Case "TRcd". (* no IH *) apply Hrcd. induction a; auto.
+      SCase "cons". destruct a as [x T]. apply Hcons. (* Can't prove P T *)
+Abort All.
+*)
+
+(** It would be nice if one did not have to specify Q at the start, 
+    but rather when it comes up in the TRcd case. *)
+(*
+Definition ty_nested_rect_plus
+  (P: ty -> Type) 
+    (fTBase : forall x : id, P (TBase x))
+    (fTArrow : forall T1 : ty, P T1 -> forall T2 : ty, P T2 -> P (TArrow T1 T2))
+    (fTRcd : forall Trb : list decl, 
+      (exists (Q: list decl -> Type),
+              (Q nil) *
+              (forall (x : id) (T : ty) (Trb : list decl), 
+                       P T -> Q Trb -> Q ((x, T) :: Trb)) *
+              (forall Trb : list decl, (Q Trb) -> P (TRcd Trb)) ???
+      ) -> P (TRcd Trb))   
+  : forall T : ty, P T := admit.
+  := fix F (T : ty) : P T :=
+     let fix G (Trb : list decl) : Q Trb :=
+         match Trb with
+           | nil => fTRcd_nil'
+           | (x,T) :: Trb' => fTRcd_cons' x T Trb' (F T) (G Trb')
+         end
+     in match T with
+       | TBase x => fTBase x
+       | TArrow T1 T2 => fTArrow T1 (F T1) T2 (F T2)
+       | TRcd Trb => fTRcd' Trb (G Trb)
+     end.
+*)
+
+
+(** *** Recursion on terms, [tm_nested_rect]
+
+    This is similar to above, except that it is dealing with terms rather than types.
+*)
+
+Definition tm_nest_rect
+  (P: tm -> Type) 
+  (Q: list def -> Type)
+    (ftrue : P ttrue)
+    (ffalse : P tfalse)
+    (fvar : forall x : id, P (tvar x))
+    (fapp : forall t1 : tm, P t1 -> forall t2 : tm, P t2 -> P (tapp t1 t2))
+    (fabs : forall (x : id) (T : ty) (t : tm), P t -> P (tabs x T t))
+    (frcd' : forall rb : list def, Q rb -> P (trcd rb))
+      (frcd_nil' : Q nil)
+      (frcd_cons' : forall (x : id) (t : tm) (rb : list def),
+                      P t -> Q rb -> Q ((Fv x t) :: rb))
+    (fproj : forall t : tm, P t -> forall x : id, P (tproj t x)) 
+    (fif : forall tb : tm, P tb -> 
+           forall tt : tm, P tt -> 
+           forall te : tm, P te -> P (tif tb tt te)) 
+  : forall t : tm, P t
+  := fix F (t : tm) : P t := 
+    let frcd_cons bxt rb := match bxt with (Fv x t) => frcd_cons' x t rb (F t) end
+    in let frcd rb := frcd' rb (list_rect Q frcd_nil' frcd_cons rb)
+    in tm_rect P ftrue ffalse fvar fapp fabs frcd fproj fif t.
+
+Tactic Notation "t_both_cases" tactic(first) ident(c) :=
+  first;
+  [ Case_aux c "ttrue" | Case_aux c "tfalse" 
+  | Case_aux c "tvar" | Case_aux c "tapp" | Case_aux c "tabs"
+  | Case_aux c "trcd" | Case_aux c "trnil" | Case_aux c "trcons"
+  | Case_aux c "tproj" | Case_aux c "tif" ].
+
+
+
+(* ###################################################################### *)
+(** ** Reduction *)
+(** *** Substitution *)
+
+(**  Coq complains when [subst] is defined with [Fixpoint ... with] 
+     as it cannot figure out that the term is not increasing in the 
+     [with] clause.  While [subst] can be defined using the custom
+     recursion defined above, in proofs it simplifies to a mess 
+     that I can't fold back up.
+     Instead, [subst] is defined with a nested fixpoint, as follows: 
+*)
+
+Reserved Notation "'[' x ':=' s ']' t" (at level 20).
+Reserved Notation "'[' x ':=' s ']*' r" (at level 20).
+
+Fixpoint subst (x:id) (s:tm) (t:tm) {struct t} : tm :=
+  let rsubst := (fix rsubst  (a: list def) : list def := 
+    match a with
+      | nil => nil 
+      | (Fv i t) :: r' => (Fv i ([x:=s] t)) :: (rsubst r')
+    end)
+  in
+  match t with
+    | ttrue => ttrue
+    | tfalse => tfalse
+    | tvar y => if eq_id_dec x y then s else t
+    | tabs y T t1 =>  tabs y T (if eq_id_dec x y then t1 else (subst x s t1))
+    | tapp t1 t2 => tapp ([x:=s] t1) ([x:=s] t2)
+    | trcd r => trcd (rsubst r)
+    | tproj t1 i => tproj ([x:=s] t1) i
+    | tif t1 t2 t3 => tif ([x:=s] t1) ([x:=s] t2) ([x:=s] t3)
+  end
+
+where "'[' x ':=' s ']' t" := (subst x s t).
+
+(**  In order to make the nested fixpoint visible, it is defined again as
+     [subst_rcd] and a lemma is given that supports rewriting the nested
+     fixpoint to it. *)
+
+Fixpoint subst_rcd (x:id) (s:tm) (a: list def) : list def := 
+  match a with
+    | nil => nil 
+    | (Fv i t) :: rb' => (Fv i ([x:=s] t)) :: ([x:=s]* rb')
+  end
+
+where "'[' x ':=' s ']*' r" := (subst_rcd x s r).
+
+
+Lemma subst_rcd_eqv :
+  forall x s a,
+    [x := s]* a =
+    ((fix rsubst (a0 : list def) : list def :=
+         match a0 with
+         | nil => nil
+         | (Fv i t) :: r' => (Fv i ([x := s]t)) :: (rsubst r')
+         end) a).
+Proof.
+  intros. induction a.
+    reflexivity.
+    simpl. rewrite <- IHa. reflexivity.
 Qed.
 
-(* ################################### *)
-(** *** Typing Relation *)
+
+(**   Here is substitution defined using the custom recursion defined above.
+      However, I don't know how to use the match syntax with a custom 
+      recursion principle, so it's not easy to read.  Further, it simplifies 
+      into a mess that I can't fold back up, so we're not using this. *)
+
+Definition subst_ugly (x:id) (s:tm) :tm -> tm := 
+  tm_nest_rect (fun _ => tm) (fun _ => list def)
+    ttrue                                               (* ttrue *)
+    tfalse                                              (* tfalse *)
+    (fun y => if eq_id_dec x y then s else (tvar y))    (* tvar y *)
+    (fun t1 mt1 t2 mt2 => tapp mt1 mt2)                 (* tapp t1 t2 *)
+    (fun y T t1 mt1 =>                                  (* tabs y T t1 *)
+       tabs y T (if eq_id_dec x y then t1 else mt1))
+    (fun r mr => trcd mr)                               (* trcd r *)
+      (nil)                                               (* nil *)
+      (fun i t r mt mr => (Fv i mt) :: mr)                (* cons i t r *)
+    (fun t1 mt1 i => tproj mt1 i)                       (* tproj t1 i *)
+    (fun tb mtb tt mtt te mte => tif mtb mtt mte)       (* tif tb tt te *)
+    .
+
+(*
+Definition tm_rect_nest (P: tm -> Type) (Q: list def -> Type)
+  (fvar : forall i : id, P (tvar i))
+  (fapp : forall t : tm,
+        P t -> forall t0 : tm, P t0 -> P (tapp t t0))
+  (fabs : forall (i : id) (t : ty) (t0 : tm),
+        P t0 -> P (tabs i t t0))
+  (fproj : forall t : tm, P t -> forall i : id, P (tproj t i))
+  (frcd : forall a : list def, Q a -> P (trcd a))
+  (frcd_nil : Q nil)
+  (frcd_cons : forall (i : id) (t : tm) (a : list def), P t -> Q a -> Q (cons i t a))
+ := fix F (t : tm) : P t := 
+  match t as t' return (P t') with
+    | tvar i => fvar i
+    | tapp t0 t1 => fapp t0 (F t0) t1 (F t1)
+    | tabs i t0 t1 => fabs i t0 t1 (F t1)
+    | tproj t0 i => fproj t0 (F t0) i
+    | trcd r => let frcd_cons' := (fun i y r' => frcd_cons i y r' (F y) )
+      in frcd r (alist_rect tm Q frcd_nil frcd_cons' r)
+  end.
+ *)
+
+
+
+(* Some other stuff: *)
+
+Fixpoint alist_all {T : Type} (P : T-> Prop) (a: alist T) : Prop :=
+  match a with
+    | nil => True
+    | (i, t) :: r => P t /\ alist_all P r
+  end.
+
+Definition tm_rect_nest_map
+  (ftrue : tm)
+  (ffalse : tm)
+  (fvar : id -> tm)
+  (fapp : tm -> tm -> tm -> tm -> tm)
+  (fabs : id -> ty ->  tm -> tm -> tm)
+  (fproj : tm -> tm -> id -> tm)
+  (fif : tm -> tm -> tm -> tm -> tm -> tm -> tm)
+ := tm_nest_rect
+      (fun _ => tm)  (fun _ => list def) ftrue ffalse fvar fapp fabs
+      (fun r mr => trcd mr) nil (fun i t r mt mr => (Fv i mt) :: mr) fproj fif.
+
+
+Definition subst'' (x:id) (s:tm) : tm -> tm := 
+  tm_rect_nest_map
+    ttrue
+    tfalse
+    (fun y => if eq_id_dec x y then s else (tvar y))
+    (fun t1 mt1 t2 mt2 => tapp mt1 mt2)
+    (fun y T t1 mt1 =>  tabs y T (if eq_id_dec x y then t1 else mt1))
+    (fun t1 mt1 i => tproj mt1 i)
+    (fun tb mtb tt mtt te mte => tif mtb mtt mte).
+
+(*
+Example subst''_ok :substf_ok subst''.
+Proof. unfold substf_ok. repeat split. Qed.
+*)
+
+Definition tm_id : tm -> tm := 
+  tm_nest_rect (fun _ => tm) (fun _ => list def)
+    ttrue 
+    tfalse
+    (fun y => tvar y)
+    (fun t1 mt1 t2 mt2 => tapp t1 t2)
+    (fun y T t1 mt1 =>  tabs y T t1)
+    (fun r mr => trcd r)
+    (nil)
+    (fun i t r mt mr => (Fv i t) :: r)
+    (fun t1 mt1 i => tproj t1 i)
+    (fun tb mtb tt mtt te mte => tif tb tt te).
+(*
+Example ex_id1 : (tm_id (tapp (tvar f) (tvar a)))
+    =  (tapp (tvar f) (tvar a)).
+Proof. reflexivity. Qed.
+*)
+
+(* ###################################################################### *)
+
+
+(** *** Values 
+<<
+       v ::=                          Values:
+           | true | false                boolean values
+           | \x:T.t                      abstractions
+           | {i1=v1, ..., in=vn}         record values
+>> 
+Note that a record is a value if all of its fields are. *)
+
+
+Inductive value : tm -> Prop :=
+  | v_true : 
+      value ttrue
+  | v_false : 
+      value tfalse
+  | v_abs : forall x T11 t12,
+      value (tabs x T11 t12)
+  | v_rcd : forall r, 
+      value_rcd r -> 
+      value (trcd r)
+
+with value_rcd : (list def) -> Prop :=
+  | vr_nil : 
+      value_rcd nil
+  | vr_cons : forall x v1 vr,
+      value v1 ->
+      value_rcd vr ->
+      value_rcd (add_vdef x v1 vr).
+
+Hint Constructors value value_rcd.
+
+
+(** *** Reduction rules
+<<
+                               value v2
+                     ----------------------------                   (ST_AppAbs)
+                     (\x:T.t12) v2 ==> [x:=v2]t12
+
+                              t1 ==> t1'
+                           ----------------                           (ST_App1)
+                           t1 t2 ==> t1' t2
+
+                              value v1
+                              t2 ==> t2'
+                           ----------------                           (ST_App2)
+                           v1 t2 ==> v1 t2'
+
+                                 t1 ==> t1'
+                               --------------                        (ST_Proj1)
+                               t1.i ==> t1'.i
+
+                          -------------------------                (ST_ProjRcd)
+                          {..., i=vi, ...}.i ==> vi
+
+                                 ti ==> ti'                            (ST_Rcd)
+    --------------------------------------------------------------------  
+    {i1=v1, ..., im=vm, in=tn, ...} ==> {i1=v1, ..., im=vm, in=tn', ...}
+
+                    --------------------------------                (ST_IfTrue)
+                    (if true then t1 else t2) ==> t1
+
+                    ---------------------------------              (ST_IfFalse)
+                    (if false then t1 else t2) ==> t2
+
+                              t1 ==> t1'
+         ----------------------------------------------------           (ST_If)
+         (if t1 then t2 else t3) ==> (if t1' then t2 else t3)
+
+>> 
+*)
+
+Reserved Notation "t1 '==>' t2" (at level 40).
+Reserved Notation "rb1 '*==>' rb2" (at level 40).
+
+Inductive step : tm -> tm -> Prop :=
+  | ST_AppAbs : forall x T11 t12 v2,
+         value v2 ->
+         (tapp (tabs x T11 t12) v2) ==> ([x:=v2]t12)
+  | ST_App1 : forall t1 t1' t2,
+         t1 ==> t1' ->
+         (tapp t1 t2) ==> (tapp t1' t2)
+  | ST_App2 : forall v1 t2 t2',
+         value v1 ->
+         t2 ==> t2' ->
+         (tapp v1 t2) ==> (tapp v1 t2')
+  | ST_Proj1 : forall t1 t1' i,
+        t1 ==> t1' ->
+        (tproj t1 i) ==> (tproj t1' i)
+  | ST_ProjRcd : forall r x vx,
+        value_rcd r ->
+        lookup_vdef x r = Some vx ->
+        (tproj (trcd r) x) ==> vx
+  | ST_Rcd : forall rb rb',
+        rb *==> rb' ->
+        (trcd rb) ==> (trcd rb')
+  | ST_IfTrue : forall t1 t2,
+        (tif ttrue t1 t2) ==> t1
+  | ST_IfFalse : forall t1 t2,
+        (tif tfalse t1 t2) ==> t2
+  | ST_If : forall t1 t1' t2 t3,
+        t1 ==> t1' ->
+        (tif t1 t2 t3) ==> (tif t1' t2 t3)
+
+with step_rcd : (list def) -> (list def) -> Prop := 
+  | STR_Head : forall x t t' rb,
+        t ==> t' ->
+        (add_vdef x t rb) *==> (add_vdef x t' rb)
+  | STR_Tail : forall x v rb rb',
+        value v ->
+        rb *==> rb' ->
+        (add_vdef x v rb) *==> (add_vdef x v rb')
+
+where "t1 '==>' t2" := (step t1 t2)
+and "rb1 '*==>' rb2" := (step_rcd rb1 rb2).
+
+Tactic Notation "step_cases" tactic(first) ident(c) :=
+  first;
+  [ Case_aux c "ST_AppAbs" | Case_aux c "ST_App1" | Case_aux c "ST_App2"
+  | Case_aux c "ST_Proj1" | Case_aux c "ST_ProjRcd" | Case_aux c "ST_Rcd" 
+  | Case_aux c "ST_IfTrue" | Case_aux c "ST_IfFalse" | Case_aux c "ST_If"].
+
+Tactic Notation "step_rcd_cases" tactic(first) ident(c) :=
+  first;
+  [ Case_aux c "STR_Head" | Case_aux c "STR_Tail" ].
+
+Notation multistep := (multi step).
+Notation "t1 '==>*' t2" := (multistep t1 t2) (at level 40).
+
+Hint Constructors step step_rcd.
+ 
+
+(* ###################################################################### *)
+(** ** Typing *)
+
+(** *** Contexts *)
+
+Definition context := list decl.
+Definition empty := nil (A:=decl).
+Definition extend (Gamma : context) (x : id) (T : ty) := (Lv x T) :: Gamma.
+
+Lemma extend_eq : forall (ctxt: context) x T,
+  lookup_vdecl x (extend ctxt x T) = Some T.
+Proof.
+  intros. unfold extend, lookup_vdecl. rewrite eq_id; auto. 
+Qed.
+
+Lemma extend_neq : forall (ctxt: context) x1 x2 T,
+  x2 <> x1 ->
+  lookup_vdecl x1 (extend ctxt x2 T) = lookup_vdecl x1 ctxt.
+Proof.
+  intros. unfold extend, lookup_vdecl. rewrite neq_id; auto. 
+Qed.
+
+
+(** *** Typing rules:
+<<
+                             Gamma x = T
+                            --------------                              (T_Var)
+                            Gamma |- x : T
+
+                      Gamma , x:T11 |- t12 : T12
+                     ----------------------------                       (T_Abs)
+                     Gamma |- \x:T11.t12 : T11->T12
+
+                        Gamma |- t1 : T11->T12
+                          Gamma |- t2 : T11
+                        ----------------------                          (T_App)
+                         Gamma |- t1 t2 : T12
+
+               Gamma |- [i1=t1, ..., in=tn] *: [1:T1, ..., in:Tn]
+             --------------------------------------------------         (T_Rcd)
+             Gamma |- {i1=t1, ..., in=tn} : {i1:T1, ..., in:Tn}
+
+                       Gamma |- t : {..., i:Ti, ...}
+                       -----------------------------                   (T_Proj)
+                             Gamma |- t.i : Ti
+
+                         --------------------                          (T_True)
+                         Gamma |- true : Bool
+
+                        ---------------------                         (T_False)
+                        Gamma |- false : Bool
+
+       Gamma |- t1 : Bool    Gamma |- t2 : T    Gamma |- t3 : T
+       --------------------------------------------------------          (T_If)
+                  Gamma |- if t1 then t2 else t3 \in : T  
+
+                        -------------------                            (TR_Nil)
+                        Gamma |- []  *:  []
+
+                           Gamma |- t : T
+                          Gamma |- tr *: Tr
+                  ---------------------------------                   (TR_Cons)
+                  Gamma |- i=t :: tr  *:  i:T :: Tr
+>> 
+*)
 
 Reserved Notation "Gamma '|-' t '\in' T" (at level 40).
+Reserved Notation "Gamma '|-' r '*\in' Tr" (at level 40).
 
 Inductive has_type : context -> tm -> ty -> Prop :=
   | T_Var : forall Gamma x T,
       lookup_vdecl x Gamma = Some T ->
       Gamma |- tvar x \in T
-  | T_Abs : forall Gamma x T11 T12 t12,
-      add_vdecl x T11 Gamma |- t12 \in T12 -> 
-      Gamma |- tabs x T11 t12 \in TArrow T11 T12
-  | T_App : forall T11 T12 Gamma t1 t2,
-      Gamma |- t1 \in TArrow T11 T12 -> 
-      Gamma |- t2 \in T11 -> 
-      Gamma |- tapp t1 t2 \in T12
+  | T_Abs : forall Gamma x T1 T2 tb,
+      (extend Gamma x T1) |- tb \in T2 -> 
+      Gamma |- (tabs x T1 tb) \in (TArrow T1 T2)
+  | T_App : forall T1 T2 Gamma t1 t2,
+      Gamma |- t1 \in (TArrow T1 T2) -> 
+      Gamma |- t2 \in T1 -> 
+      Gamma |- (tapp t1 t2) \in T2
+  | T_Rcd : forall Gamma tr Tr,
+      Gamma |- tr *\in Tr ->
+      Gamma |- (trcd tr) \in (TRcd Tr)
+  | T_Proj : forall Gamma x t Tx Tr,
+      Gamma |- t \in (TRcd Tr) ->
+      lookup_vdecl x Tr = Some Tx ->
+      Gamma |- (tproj t x) \in Tx
   | T_True : forall Gamma,
        Gamma |- ttrue \in TBool
   | T_False : forall Gamma,
@@ -213,17 +726,41 @@ Inductive has_type : context -> tm -> ty -> Prop :=
        Gamma |- t3 \in T ->
        Gamma |- tif t1 t2 t3 \in T
 
-where "Gamma '|-' t '\in' T" := (has_type Gamma t T).
+with rcd_has_type : context -> (list def) -> (list decl) -> Prop :=
+  | TR_Nil : forall Gamma,
+      Gamma |- nil *\in nil
+  | TR_Cons : forall Gamma x t T tr Tr,
+      Gamma |- t \in T ->
+      Gamma |- tr *\in Tr ->
+      Gamma |- (add_vdef x t tr) *\in (add_vdecl x T Tr)
+
+where "Gamma '|-' t '\in' T" := (has_type Gamma t T)
+and   "Gamma '|-' r '*\in' Tr" := (rcd_has_type Gamma r Tr).
+
+Hint Constructors has_type rcd_has_type.
 
 Tactic Notation "has_type_cases" tactic(first) ident(c) :=
   first;
-  [ Case_aux c "T_Var" | Case_aux c "T_Abs" 
-  | Case_aux c "T_App" | Case_aux c "T_True" 
-  | Case_aux c "T_False" | Case_aux c "T_If" ].
+  [ Case_aux c "T_Var" | Case_aux c "T_Abs" | Case_aux c "T_App"
+  | Case_aux c "T_Rcd" | Case_aux c "T_Proj" 
+  | Case_aux c "T_True" | Case_aux c "T_False" | Case_aux c "T_If" ].
 
-Hint Constructors has_type.
+Tactic Notation "rcd_has_type_cases" tactic(first) ident(c) :=
+  first;
+  [ Case_aux c "TR_Nil" | Case_aux c "TR_Cons" ].
+
+(** *** Custom induction principle for typing *)
+
+Scheme has_type_ind_both := Minimality for has_type Sort Prop
+with rcd_has_type_ind_both := Minimality for rcd_has_type Sort Prop.
+
+Tactic Notation "has_type_both_cases" tactic(first) ident(c) :=
+  first;
+  [ Case_aux c "T_Var" | Case_aux c "T_Abs" | Case_aux c "T_App"
+  | Case_aux c "T_Rcd" | Case_aux c "T_Proj" 
+  | Case_aux c "T_True" | Case_aux c "T_False" | Case_aux c "T_If"
+  | Case_aux c "TR_Nil" | Case_aux c "TR_Cons" ].
+
+
 
 End LDEF.
-
-(** $Date: $ *)
-
