LEProps3.v
@@ -10,8 +10,8 @@ Load Init.
 Require Export SfLib.
 Require Import LibTactics.
 
-Require Export Common RecordsExt LEval.
-Import P3Common Records LEVAL.
+Require Export Common LDef LEval.
+Import P3Common LDEF LEVAL.
 
 Module LEProps3.
 
