Makefile
@@ -1,4 +1,4 @@
-MODULES := Common LDef LProps LEval Tests Tests2 LEProps LEProps3 Utils RecordsExt TestsR
+MODULES := Common Utils LDef LProps OLDef OLProps LEval LEProps LEProps3 Tests Tests2 TestsR
 VS      := $(MODULES:%=%.v)
 PSF			:= ../../Coq/pierce_software_foundations_3.2
 
@@ -10,9 +10,11 @@ coq: Makefile.coq
 Makefile.coq: Makefile
 	coq_makefile -I . -I $(PSF) $(VS) -o Makefile.coq
 
-clean:: Makefile.coq
-	$(MAKE) -f Makefile.coq clean
-	rm -f Makefile.coq
+# clean:: Makefile.coq
+# 	$(MAKE) -f Makefile.coq clean
+# 	rm -f Makefile.coq
+clean:
+	rm -f Makefile.coq *.v.d *.vo *.glob
 
 html:: Makefile.coq
 	$(MAKE) -f Makefile.coq html
